pulse/share/steel/examples/pulse/lib/Pulse.Lib.Coinduction.fst
@@ -1,0 +1,236 @@
+module Pulse.Lib.Coinduction
+
+open Steel.Memory
+
+#push-options "--print_universes"
+
+unfold
+let inner_gfp #a (f: pred a -> pred a) (x: a) (p: pred a)
+= h_and (p x) (pure (implies p (f p)))
+
+let h_and_equiv (p q: slprop) (m:mem)
+  : Lemma ((interp p m /\ interp q m) <==> interp (h_and p q) m)
+= elim_h_and p q m; intro_h_and p q m
+
+let inner_gfp_equiv
+#a (f: pred a -> pred a) (x: a) (p: pred a) m
+: Lemma (
+    interp (inner_gfp f x p) m 
+    <==> interp (p x) m /\ implies p (f p)
+)
+= h_and_equiv (p x) (pure (implies p (f p))) m;
+  pure_interp (implies p (f p)) m
+
+let gfp_sat_aux #a (f: pred a -> pred a) m x:
+Lemma ((exists p. interp (p x) m /\ implies p (f p) ) <==> interp (gfp f x) m)
+= introduce forall p. ((interp (p x) m /\ implies p (f p)) ==> interp (gfp f x) m) with (
+    inner_gfp_equiv f x p m;
+    intro_h_exists p (
+        fun p -> h_and (p x) (pure (implies p (f p)))
+    ) m
+);
+introduce interp (gfp f x) m ==> (exists p. interp (p x) m /\ implies p (f p) )
+with _. (
+    elim_h_exists (
+        fun p -> h_and (p x) (pure (implies p (f p)))
+    ) m;
+    introduce forall p.
+    (
+        interp (inner_gfp f x p) m ==> (interp (p x) m /\ implies p (f p) )
+    )
+    with (
+        inner_gfp_equiv f x p m
+    )
+)
+
+let gfp_sat #a (f: pred a -> pred a):
+Lemma (forall m x. (exists p. interp (p x) m /\ implies p (f p) ) <==> interp (gfp f x) m)
+=  introduce forall m x. ((exists p. interp (p x) m /\ implies p (f p) ) <==> interp (gfp f x) m)
+with (gfp_sat_aux f m x)
+
+let set_D #a (f: pred a -> pred a) (p: pred a)
+= (implies p (f p))
+
+
+let in_D_implies_than_u #a (f: mono_fun a) p
+: Lemma (requires set_D f p)
+    (ensures implies p (gfp f))
+= gfp_sat f
+
+let lemma_D_aux #a (f: mono_fun a) p
+: Lemma (requires set_D f p)
+        (ensures implies p (f (gfp f)))
+= 
+let u = gfp f in
+  in_D_implies_than_u f p;
+  assert (implies (f p) (f u))
+
+let lemma_D #a (f: mono_fun a)
+: Lemma (forall p. set_D f p ==> implies p (f (gfp f)))
+=
+introduce forall p. (set_D f p ==> implies p (f (gfp f)))
+with (
+    introduce set_D f p ==> implies p (f (gfp f))
+    with _. lemma_D_aux f p)
+
+let gfp_implies_than_itself
+    #a (f: mono_fun a)
+: Lemma// (implies (gfp f) (f (gfp f)))
+    (forall m x. interp (gfp f x) m ==> interp (f (gfp f) x) m)
+= gfp_sat f; lemma_D f
+
+let lemma_u_in_D #a (f: mono_fun a)
+: Lemma (set_D f (gfp f))
+= gfp_implies_than_itself f 
+
+// Knaster-Tarski theorem
+let gfp_is_fixed_point #a (f: mono_fun a)
+    //Lemma (equivalent (gfp f) (f (gfp f)))
+= gfp_implies_than_itself f; in_D_implies_than_u f (f (gfp f))
+
+let gfp_is_largest_fp #a (f: mono_fun a) p
+//:
+//Lemma (requires equivalent p (f p))
+//(ensures implies p (gfp f))
+= gfp_sat f
+
+let gfp_is_fixed_point_eq #a (f: mono_fun a):
+    Lemma (forall x. gfp f x == f (gfp f) x)
+= introduce forall x. (gfp f x == f (gfp f) x)
+with (
+    gfp_is_fixed_point f;
+    //reveal_equiv (gfp f x) (f (gfp f) x);
+    slprop_extensionality (gfp f x) (f (gfp f) x)
+)
+
+let coinduction #a (f: mono_fun a) (p: pred a):
+    Lemma (requires implies p (f p))
+    (ensures implies p (gfp f))
+= gfp_sat f
+
+let interp_rec_forall_def ty f x delta
+: Lemma (interp_rec (Forall ty f) delta x == h_forall (fun y -> interp_rec (f y) delta x))
+= assert_norm (interp_rec (Forall ty f) delta x == h_forall (fun y -> interp_rec (f y) delta x))
+
+let interp_rec_exists_def ty f x delta
+: Lemma (interp_rec (Exists ty f) delta x == h_exists (fun y -> interp_rec (f y) delta x))
+= assert_norm (interp_rec (Exists ty f) delta x == h_exists (fun y -> interp_rec (f y) delta x))
+
+let h_and_equiv_forall (p q: slprop):
+    Lemma (forall m. interp (h_and p q) m <==> (interp p m /\ interp q m))
+= introduce forall m. interp (h_and p q) m <==> (interp p m /\ interp q m)
+  with h_and_equiv p q m
+
+let h_or_equiv_forall (p q: slprop):
+    Lemma (forall m. interp (h_or p q) m <==> (interp p m \/ interp q m))
+= introduce forall m. (interp (h_or p q) m <==> (interp p m \/ interp q m))
+with (
+    elim_h_or p q m;
+    intro_h_or_left p q m;
+    intro_h_or_right p q m
+)
+
+let h_exists_equiv_forall p:
+    Lemma (forall m. interp (h_exists p) m <==> (exists x. interp (p x) m))
+= introduce forall m. (interp (h_exists p) m <==> (exists x. interp (p x) m))
+  with (
+    elim_h_exists p m;
+    introduce forall w. (interp (p w) m ==> interp (h_exists p) m)
+    with intro_h_exists w p m
+  )
+
+let h_forall_equiv p m:
+    Lemma (interp (h_forall p) m <==> (forall x. interp (p x) m))
+= intro_h_forall p m; 
+  introduce forall x. (interp (h_forall p) m ==> interp (p x) m)
+  with elim_h_forall p m x
+
+let h_forall_equiv_forall p:
+    Lemma (forall m. interp (h_forall p) m <==> (forall x. interp (p x) m))
+= introduce forall m. (interp (h_forall p) m <==> (forall x. interp (p x) m))
+  with h_forall_equiv p m
+
+let star_equiv_forall p q:
+    Lemma (forall m.
+  (interp (p `star` q) m <==>
+  (exists (mp: mem) (mq: mem) . disjoint mp mq /\ interp p mp /\ interp q mq /\ join mp mq == m)))
+= introduce forall m.
+    (interp (p `star` q) m <==>
+    (exists (mp: mem) (mq: mem) . disjoint mp mq /\ interp p mp /\ interp q mq /\ join mp mq == m))
+  with interp_star p q m
+
+let wand_equiv_forall p q:
+    Lemma (forall m.
+    (interp (p `wand` q) m <==>
+    (forall mp.
+        disjoint m mp /\
+        interp p mp ==>
+        interp q (join m mp))))
+= introduce forall m.
+    (interp (p `wand` q) m <==>
+    (forall mp.
+        disjoint m mp /\ interp p mp ==> interp q (join m mp)))
+with (
+    intro_wand p q m;
+    introduce forall m1. ((interp (wand p q) m /\ m `disjoint` m1 /\ interp p m1)
+    ==> interp q (join m m1))
+    with (
+        elim_wand p q m m1
+    )
+)
+
+let rec interp_rec_mono_aux #a (r: rec_def a) (p q: pred a) (x: a):
+    Lemma (requires forall x. slimp (p x) (q x))
+        (ensures slimp (interp_rec r p x) (interp_rec r q x))
+= match r with
+| And r1 r2 ->
+    h_and_equiv_forall (interp_rec r1 p x) (interp_rec r2 p x);
+    h_and_equiv_forall (interp_rec r1 q x) (interp_rec r2 q x);
+    interp_rec_mono_aux r1 p q x;
+    interp_rec_mono_aux r2 p q x
+| Or r1 r2 ->
+    h_or_equiv_forall (interp_rec r1 p x) (interp_rec r2 p x);
+    h_or_equiv_forall (interp_rec r1 q x) (interp_rec r2 q x);
+    interp_rec_mono_aux r1 p q x;
+    interp_rec_mono_aux r2 p q x
+| Forall ty fr ->
+    introduce forall y. (slimp (interp_rec (fr y) p x) (interp_rec (fr y) q x))
+        with (interp_rec_mono_aux (fr y) p q x);
+    interp_rec_forall_def ty fr x p;
+    interp_rec_forall_def ty fr x q;
+    h_forall_equiv_forall (fun y -> interp_rec (fr y) p x);
+    h_forall_equiv_forall (fun y -> interp_rec (fr y) q x)
+| Exists ty fr ->
+    introduce forall y. (slimp (interp_rec (fr y) p x) (interp_rec (fr y) q x))
+        with (interp_rec_mono_aux (fr y) p q x);
+    interp_rec_exists_def ty fr x p;
+    interp_rec_exists_def ty fr x q;
+    h_exists_equiv_forall (fun y -> interp_rec (fr y) p x);
+    h_exists_equiv_forall (fun y -> interp_rec (fr y) q x)
+| SLProp _ -> ()
+| RecursiveCall f -> ()
+| Star r1 r2 -> 
+    star_equiv_forall (interp_rec r1 p x) (interp_rec r2 p x);
+    star_equiv_forall (interp_rec r1 q x) (interp_rec r2 q x);
+    interp_rec_mono_aux r1 p q x;
+    interp_rec_mono_aux r2 p q x
+| Wand f r' ->
+    wand_equiv_forall (f x) (interp_rec r' p x);
+    wand_equiv_forall (f x) (interp_rec r' q x);
+    interp_rec_mono_aux r' p q x
+
+let interp_rec_mono #a (r: rec_def a):
+    Lemma (mono (interp_rec r))
+= introduce forall p q x.
+  ((forall x. slimp (p x) (q x)) ==> slimp (interp_rec r p x) (interp_rec r q x))
+  with (
+    introduce (forall x. slimp (p x) (q x)) ==> slimp (interp_rec r p x) (interp_rec r q x)
+    with _. interp_rec_mono_aux r p q x
+  )
+
+let interp_rec_fold_unfold #a (p: rec_def a):
+    Lemma (forall x. gfp (interp_rec p) x == interp_rec p (gfp (interp_rec p)) x)
+= interp_rec_mono p; gfp_is_fixed_point_eq (interp_rec p)
+
+let coinduction_principle (#a: Type) (r: rec_def a) (p: pred a)
+= interp_rec_mono r; coinduction (interp_rec r) p
