pulse/share/steel/examples/pulse/lib/Pulse.Lib.Coinduction.fsti
@@ -1,0 +1,111 @@
+module Pulse.Lib.Coinduction
+
+open Steel.DisposableInvariant
+open Steel.Memory
+
+type pred a = (a -> slprop)
+
+let implies #a (p q: pred a) = (forall x. slimp (p x) (q x))
+
+let mono #a (f: pred a -> pred a) =
+    (forall p q x. (forall y. slimp (p y) (q y)) ==> slimp (f p x) (f q x))
+
+let mono_fun a = (f: (pred a -> pred a){mono f})
+
+let gfp #a (f: pred a -> pred a): pred a
+= (fun x -> (h_exists (fun p -> h_and (p x) (pure (implies p (f p))))))
+// x -> (exists (p:slprop). p x /\ p ==> f p)
+
+// Knaster-Tarski theorem
+val gfp_is_fixed_point (#a: Type) (f: mono_fun a):
+    Lemma (forall x. equiv (gfp f x) (f (gfp f) x))
+
+val gfp_is_largest_fp (#a: Type) (f: mono_fun a) (p: pred a):
+    Lemma (requires forall x. equiv (p x) (f p x))
+          (ensures forall x. (slimp (p x) (gfp f x)))
+
+val gfp_is_fixed_point_eq (#a: Type) (f: mono_fun a):
+    Lemma (forall x. gfp f x == f (gfp f) x)
+
+// one can prove that any element satisfying p also satisfies gfp f
+// as long as f preserves p (p ==> f p)
+val coinduction (#a: Type) (f: mono_fun a) (p: pred a):
+    Lemma (requires implies p (f p))
+    (ensures implies p (gfp f))
+
+noeq
+type rec_def (a: Type) =
+| Star: rec_def a -> rec_def a -> rec_def a
+| And: rec_def a -> rec_def a -> rec_def a
+| Or: rec_def a -> rec_def a -> rec_def a
+| Wand: (a -> slprop) -> rec_def a -> rec_def a // prevents contravariant recursion
+| RecursiveCall: (a -> a) -> rec_def a
+| SLProp: (a -> slprop) -> rec_def a
+| Exists: t:Type0 -> (t -> rec_def a) -> rec_def a
+| Forall: t:Type0 -> (t -> rec_def a) -> rec_def a
+
+let rec interp_rec #a (r: rec_def a) (delta: pred a): pred a
+= fun x -> (
+    match r with
+    | Star r1 r2 -> star (interp_rec r1 delta x) (interp_rec r2 delta x)
+    | And r1 r2 -> h_and (interp_rec r1 delta x) (interp_rec r2 delta x)
+    | Or r1 r2 -> h_or (interp_rec r1 delta x) (interp_rec r2 delta x)
+    | Wand f r' -> wand (f x) (interp_rec r' delta x)
+    | RecursiveCall f -> delta (f x)
+    | SLProp f -> f x
+    | Exists ty f -> h_exists (fun y -> interp_rec (f y) delta x)
+    | Forall ty f -> h_forall (fun y -> interp_rec (f y) delta x)
+)
+
+val interp_rec_mono (#a: Type) (r: rec_def a):
+    Lemma (mono (interp_rec r))
+
+let coinduct (#a: Type) (r: rec_def a): pred a
+= gfp (interp_rec r)
+
+val interp_rec_fold_unfold (#a: Type) (r: rec_def a):
+    Lemma (forall x. coinduct r x == interp_rec r (coinduct r) x)
+
+val coinduction_principle (#a: Type) (r: rec_def a) (p: pred a):
+    Lemma (requires implies p (interp_rec r p))
+    (ensures implies p (coinduct r))
+
+module R = Steel.Reference
+open Steel.FractionalPermission
+
+noeq
+type cell (a: Type0) = {
+    v: a;
+    next: R.ref (cell a)
+}
+
+#set-options "--print_universes"
+
+// stream(x) = exists v. x |-> v ** stream(v)
+let rec_stream a //(f: nat -> ref int) =
+: rec_def (R.ref (cell a))
+= Exists _ (fun v -> Star (SLProp (fun x -> R.pts_to_sl x full_perm v))
+    (RecursiveCall (fun _ -> v.next)))
+
+// stream(x) = exists v. x -> v ** stream(v.next)
+
+//let coinduct (#a: Type) (r: rec_def a): pred a
+let stream a: pred (R.ref (cell a)) = coinduct (rec_stream a)
+
+let interp_rec_exists_def ty f x delta
+: Lemma (interp_rec (Exists ty f) delta x == h_exists (fun y -> interp_rec (f y) delta x))
+= assert_norm (interp_rec (Exists ty f) delta x == h_exists (fun y -> interp_rec (f y) delta x))
+
+let interp_rec_fold_unfold_stream (a: Type) (r: rec_def a) (x:R.ref(cell a)) :
+    Lemma (stream a x == h_exists (fun v -> R.pts_to_sl x full_perm v `star` stream a (v.next)))
+= 
+    calc (==) {
+        stream a x;
+        == { interp_rec_fold_unfold (rec_stream a) }
+        interp_rec (rec_stream a) (stream a) x;
+        == { }
+         interp_rec (Exists _ (fun v -> Star (SLProp (fun x -> R.pts_to_sl x full_perm v))
+        (RecursiveCall (fun _ -> v.next)))) (stream a) x;
+        == { _ by (Tactics.compute ()) }
+        h_exists (fun v -> R.pts_to_sl x full_perm v `star` stream a (v.next));
+    }
